Avoid failures with function/non-equality types
Function types passed to datatype constructors mean that
EqualityType and IsTypeRep are (probably) impossible. However,
the provers now handle these datatypes normally, although the
saved theorems have (probably) impossible preconditions.

translator/ml_translatorScript.sml
@@ -478,7 +478,7 @@ Proof
 QED
 
 Definition UNIT_v_def:
-  UNIT_v (u:unit) = (Conv NONE [])
+  UNIT_v (u : unit) = (Conv NONE [])
 End
 
 Definition INT_v_def:
@@ -544,6 +544,10 @@ Proof
   \\ fs [IsTypeRep_def]
 QED
 
+Definition FUN_TYPE_REP_v:
+  FUN_TYPE_REP_v (a_v : 'a -> v) (b_v : 'b -> v) (f : 'a -> 'b) = UNIT_v ()
+End
+
 Theorem IsTypeRep_NUM_BOOL:
   IsTypeRep NUM_v NUM /\ IsTypeRep INT_v INT /\
   IsTypeRep BOOL_v BOOL /\
@@ -551,9 +555,10 @@ Theorem IsTypeRep_NUM_BOOL:
   IsTypeRep UNIT_v UNIT_TYPE /\
   IsTypeRep STRING_v STRING_TYPE /\
   IsTypeRep HOL_STRING_v HOL_STRING_TYPE /\
+  (F ==> IsTypeRep (FUN_TYPE_REP_v a_v b_v) (a --> b)) /\
   (dimindex (:'a) <= 64 ==> IsTypeRep WORD_v (WORD : 'a word -> v -> bool))
 Proof
-  EVAL_TAC \\ simp []
+  simp [] \\ EVAL_TAC \\ simp []
   \\ rpt (conj_tac ORELSE disch_tac)
   \\ Cases
   \\ EVAL_TAC
